h_i^j (n) =  P_i(T_j=n) = f_ij^n

To Prove:
pij^n = sum f_ij^m pjj^(n-m)

Proof:
pij^n = P_i(X_n = j) = P(X_n=j | X_0=i)
        = sum_m=1^n P_i (X_n=j, T_j=m)
        = sum_m=1^n P_i (X_n=j| T_j=m)P(T_j = m)
        = sum_m=1^n f_ij^m P(T_j = m)
        = sum_m=1^n f_ij^m p_jj^(n-m) } from SMP

Define N_i = Sum_k=1^infty TT_{X_n = i} = no of visits to state i

Proposition:
P_i(N_j = k) = {
    1 - f_ij for k=0
    f_ij (1-f_jj) f_jj^k-1 for k>0
}
Where f_ij = P_i(T_j < infty).

For k = 0,
P_i(N_j = 0) = P_i(T_j = infty)
            = 1- P_i(T_j < infty)
            = 1 - f_ij

For k>0
Proof by induction:
P_i(N_j = k)    = P_i(T_j^k+1 - T_j^k = infty, T_j < infty)
                = P_i(T_j^k+1 - T_j = infty | T_j^k < infty) P_i(T_j^infty < infty)
                = P_j(T_j = infty) P_i(T_j^k < infty)
                = (1 - f_jj) P_i(T_j^k < infty)
                = (1-f_jj) P_i(N_j >= k)
                = (1 -f_jj) (1 - sum_r=0^k-1 P_i(N_j = r))
                = (1 -f_jj) (1 - [1 - f_ij + sum_r=0^k-1 f_ij (1-fjj) f_jj^{r-1} ]) from induction hypothesis
                = (1 -f_jj) (f_ij - f_ij (f_jj^0 - f_jj^k-1))
                = (1 - f_jj) (f_ij f_jj^k-1)

P_i(N_i >= k) ?=

# Recurrence and Transience of a Markov Chain

i in S is called recurrent if P(X_n = i for infinitely many n) = 1

it is called transient if P(X_n = i for infinitely many n) = 0

Theorem: TFAE
1. i in S is recurrent
2. f_ii = 1
3. P_i(N_i = infinity) = 1
4. E_i[N_i] = infinity
5. sum_n p_ii^(n) = infty

1 <=> 3 by defn
3 ==> 4 is obvious
4 ==> 3 requires the fact that N_i ~ Geom(f_ii) => P_i(N_i = infty) = 1
1 <=> 2 f_ii = P_i(T_i < infty) = 1; so if P(X_n = i) = 1 for some n, it must hit i again in finite time.
4 <=> 5 E_i[sum_n=1^infty I_{X_n = i}] = sum_n P_i(X_n = i) = sum_n p_ii^n

Theorem: TFAE
1. i in S is transient
2. f_ii < 1
3. P_i(N_i < infinity) = 1
4. E_i[N_i] < infinity
5. sum_n p_ii^(n) < infinity
In particular, i transient => p_ii^(n) -> 0

Proposition: If j is transient then p_ij^(n) -> 0 as n -> infty.

Recall 
pij^n   = sum_{m=1}^n f_ij^m pjj^(n-m)
sum_n pij^n = sum_n sum_{m=1}^n f_ij^m pjj^(n-m)
            = sum_m f_ij^(m) sum_{n=m}^infty p_jj^(n-m)
            = (1 - E_j[N_j]) sum_m=1^infty f_ij^(m)
            = (1 - E_j[N_j]) P_i(T_j < infty)
            < infty

=> p_ij^n -> 0 as n -> infty

## Transience is a class property

Let i in S be transient. C be communicating class of i and take j in C.

there exists n,m st pij^(n), pji^(m) > 0

forall r >= 0; p_ii(n+r+m) >= p_ij^n p_jj^r p_ji^m

sum_r^infty p_jj^(r) <= 1/(p_ii^n p_ji^m) sum_r=0^infty p_ii^(n+r+m) < infty because i is transient.

=> p_jj^(r) -> 0 as r -> infty.

Hence, j is also transient.

## Recurrent classes are closed

Let i in C; C not closed.

Then exists j st i -> j; j -/-> i;

Then exists m st p_ij^(m) > 0;

P_i(X_n = i, X_m = j) = P_i(X_n = i | X_m = j) P_i(X_m = j) = 0

P_i(X_n = i for infinitely many n)  = P_i(A_n) 
                                    = P_i({X_m = j} CAP A_n) + P_i({X_m != j} CAP A_n)
                                    = P_i({X_m != j} CAP A_n)
                                    <= P_i(X_m != j) = 1 - P_i(X_m = j) < 1

Therefore i is not recurrent.

## Positive Recurrence and Null Recurrence

$i \in S$, $i$ recurrent, is positive recurrent if $E_i[T_i] < \infty$
$i \in S$, $i$ recurrent, is null recurrent if $E_i[T_i] = \infty$

### Connection with the stationary distribution

Aim: 

1. Irreducability + Recurrence => balance equation is satisfied
2. Irreducability + Positive Recurrence => normalization is satisfied

### Harmonic Functions

$h : S -> RR$ is a harmonic wrt to P where P is row stochastic if $h(x) = sum_{y\in S} p_{xy} h(y)$

If P is irreducable, h is a constant function. 

Since S is finite, h attains maximum at some point say $x_0$

$h(x_0) >= h(x) \forall x \in S$

Let z in S, st p_(x_0z) > 0 and suppose h(z) < h(x_0).

h(x_0) = sum_x in S p_x0x h(x) = p_x0z h(z) + sum_x!=z p_{x_0 x} h(x) < h(x_0) sum_{x in S} p_x0x = h(x_0)

That means, h(z) >= h(x_0) => h(z) = h(x_0)

Now show that any z' in S, Then exists PATH x_0 -> z', and h(k) = h(x_0) for each successive $k$.

If P h = h
(P - I) h = 0

h = cI 
=> dim(Ker(P-I)) = 1
=> dim(Ker(P^T-I)) = 1
=> (P^T - I) v^T = 0 has 1 dimensional solution
=> vP = v has 1 dimensional solution.

Hence any pi P = pi has to a constant multiple of v.

But due to normalization there is only one invariant probability distribution, 

pi = v

## Existance and Uniqueness of invariant measure

Def: Y_i^a = E[sum_n=0^{T_a - 1} I_{X_n = i}]

Thm:
Let MC(P) be irreducable and recurrent, the following hold

1. Y_a^a = 1
2. Y^a P = Y^a, where Y^a = (Y^a_i)
3. $0 < Y_i^a < \infty \forall i \in S$

1 is obvious.

Y_i^a   = E_a[sum_n=0^T_a-1 I_{X_n = i}]
        = E_a[sum_m=1^infty sum_n=0^{m-1} I_{X_n = i, T_a = m}]
        = E_a[sum_n=1^{infty} I_{X_n = i, T_a >= n}]       ------------------------ (1)
        = sum_n=1^infty sum_j P_a(X_n=i, X_{n-1} =j, T_a >= n)
        = sum_n=1^infty sum_j P_a(X_n=i | X_{n-1} =j, T_a >= n) P_a(X_m=j, T_a >= n)
        = sum_n=1^infty sum_j p_{ji} P_a(X_{n-1}=j, T_a >= n)

sum_n=1^infty P(X_{n-1}=j, T_a >= n) 
    = E_a[sum_{n=1}^infty I_{X_n-1 = j, T_a>=n}]
    = E_a[sum_{n=0}^infty I_{X_n = j, T_a>=(n+1)}]
    = Y_j^a

Hence, 2 holds

3. For i in S exists n1, n2 > 0 st

p_ia^(n1), p_ai^(n2) > 0

Y^aP^n = Y^a
=> Y_i^a >= p_ai^(n_2) Y_a^a > 0 

Thm: If lambda is invariant measure of irr MC, lambda_a = 1 for some a. Then lambda >= Y^a. If chain is also recurrent,
lambda = Y^a

lambda P = lambda

lambda_j = sum p_i0j lambda_i0 = sum_i0!=a p_i0j + p_aj lambda_a
    = sum_i0!=a p_i0j sum_i1 pi1i0 lambda_i1  + p_aj lambda_a
    = sum_i0!=a p_i0j sum_i1!=a pi1i0 lambda_i1  + sum_i0!=a p_i0j p_ai0 lambda_a + p_aj lambda_a
    = [sum_i0!=a ... sum_i_n-1!=a   ] ------------------------------- (2)
        + p_aj lambda_a 
        + sum_i0!=a p_ai0 pi_0j lambda_a
        + sum_i1!=a sum_i0!=a p_ai1 pi1i0 pi_0j lambda_a
        + ...

(2) >= 0, and hence, 

lambda_j    >= lambda_a [p_aj + sum_i0!=a p_ai0 p_i0j  ...]
            = P_a(X1=j, T_a>=1) + P_a(X2=j, T_a>=2) + ...
            = Y_j^a ------------------------------- from (1)

If chain is recurrent, 
Define mu_j = lambda_j - lambda_a Y_j^a 

mu_a = 0 
