---
title: Poisson Processes
author: Dhruva Sambrani
date: \today
geometry: margin=1in
---

# Poisson Processes

## Definition 1

Let $N(t)$ be a counting process. If

1. $N(t)$ has Independent increments
2. $P(N(t+s) - N(s) = n) = \frac{e^{-\lambda t} (\lambda t)^n}{n!} \forall S \ge 0 \text{ some } \lambda > 0$

then it is a Poisson Process.

## Definition 2

Let there be a counting process $N(t)$ such that 

1. $N(0) = 0$
2. Independent increments
3. $P(N(t) = 1) = \lambda t + o(t)$
4. $P(N(t) >= 2) = o(t)$

**Theorem:** The definitions are equivalent.

**Proof:**

(1) $\implies$ (2) is obvious from taking the taylor expansion.

Define $p_n(t) = P(N(t) = n)$

For $n = 0$,

$$\begin{aligned}
p_0(t+h) = P(N(t+h) = 0) &= P(N(t) = 0, N(t+h) - N(t) = 0)\\
&= P(N(t)) + P(N(t+h) - N(t) = 0) \leftarrow \text{  from independance}\\
&= p_0(t)(1 - (P(N(t)=1) + P(N(t) >= 2))\\
&= p_0(t)(1 - (\lambda h + o(h)))\\
\end{aligned}$$

$$\implies \frac{p_0(t+h) - p_0(t)}{h} = -\lambda p_0 + o(h)/h$$

$$\implies \frac{d p_0}{d t} = -\lambda p_0$$

$p_0 = e^{-\lambda t}$

For $n \ne 0$,

$$\begin{aligned}
p_n(t+h) =& P(N(t+h) = n, N(t) = n) \\
&+ P(N(t+h) = n, N(t) = n-1) \\
&+ P(N(t+h) = n, N(t) = n-2) + \dots \\
=& p_n(t)(1-\lambda h) + p_{n-1}(t) \lambda h + 0
\end{aligned}$$

$$\implies \frac{p_n(t+h) - p_n(t)}{h} = -\lambda (p_n(t) - p_{n-1}(t))$$

$$\frac{d p_n}{d t} = -\lambda (p_n -p_{n-1})$$

Now using the poisson distribution as an ansatz and induction, we can prove

$$\begin{aligned}
\frac{d p_1}{d t} &= -\lambda (p_1 -p_0)\\
&= - \lambda p_1 + \lambda e^{-\lambda t}
\end{aligned}$$

$$\implies p_1^\prime(t) + \lambda p_1(t) = \lambda e^{-\lambda t}$$

One can solve using Linear differential equation using I.F.


## Inter-arrival times

1. $\{X_i\}$ are i.i.d with distribution $\text{Exp}(\lambda)$
2. $P(X_1 < s | N(t)=1) = s/t I_{s < t} + I_{s > t}$

$$\begin{aligned}
P(X_1 > y) &= P(N(y) = 0)\\
           &= e^{-\lambda t}
\end{aligned}$$

$$\bar{F}(x) = 1- F(x) = 1- P(X_1 > x)$$

It is easy to show that $\bar{F}(x+h) = \bar{F}(x)\bar{F}(h)$, which is the memorylessness property
